extraction/Interop.ml
@@ -2,28 +2,3 @@ module Common = struct
   let parse_hex ls =
     int_of_string ("0x" ^ (String.concat "" (List.map (fun c -> String.make 1 c) ls)))
 end
-
-module Utf16 = struct
-  include Encoding.Utf16
-
-  let code_points_to_string (c: Encoding.codepoint list): character list = List.flatten (List.map chars_from_int c)
-
-  let to_upper_case (c: Encoding.codepoint): Encoding.codepoint list =
-    if Uchar.is_valid c then
-      match Uucp.Case.Map.to_upper (Uchar.of_int c) with
-        | `Self -> c :: []
-        | `Uchars ls -> List.map Uchar.to_int ls
-    else c :: []
-end
-
-module Unicode = struct
-  include Encoding.Unicode
-
-  let case_fold (c: character): character = 
-    if (Uchar.is_valid c) then
-      match Uucp.Case.Fold.fold (Uchar.of_int c) with
-        | `Self -> c
-        | `Uchars (cp :: []) -> Uchar.to_int cp
-        | `Uchars _ -> c
-    else c
-end
