extraction/Printers.ml
@@ -2,7 +2,8 @@ open Engines
 open Patterns
 
 module Printer(P: EngineParameters) = struct
-  open Extracted.Notation
+  type ocaml_string = string
+  open Engine(P)
 
   type character = P.character
 
@@ -11,20 +12,20 @@ module Printer(P: EngineParameters) = struct
 
     (* Regex printers *)
 
-    let prio (s: string) (at: int) (current: int) : string =
+    let prio (s: ocaml_string) (at: int) (current: int) : ocaml_string =
       if at < current then "(?:" ^ s ^ ")" else s
 
     (* TODO: check spec and update list *)
     let escaped = CS.of_list (List.map Char.code ('\\' :: '/' :: '-' :: '[' :: ']' :: '{' :: '}' :: '(' :: ')' :: '*' :: '+' :: '?' :: '$' :: '^' :: '|' :: '.' :: []))
 
-    let escape (c: character) : string =
+    let escape (c: character) : ocaml_string =
       let str = P.String.to_host (P.String.list_to_string (c :: [])) in
       if String.length str != 1 then
         failwith "Unexpected escape corner case: '" ^ str ^ "'"
       else
         "\\" ^ str
 
-    let char_lit_to_string (c: character) : string =
+    let char_lit_to_string (c: character) : ocaml_string =
       let i = P.Character.numeric_value c in
       if CS.mem i escaped then
         escape c
@@ -32,11 +33,11 @@ module Printer(P: EngineParameters) = struct
         let str = P.String.to_host (P.String.list_to_string (c :: [])) in
         str
 
-    let hex4digits_to_string (h: Extracted.HexDigit.coq_Hex4Digits) : string =
+    let hex4digits_to_string (h: Extracted.HexDigit.coq_Hex4Digits) : ocaml_string =
       let Coq_hex4 (h1, h2, h3, h4) = h in
       (String.make 1 h1) ^ (String.make 1 h2) ^ (String.make 1 h3) ^ (String.make 1 h4)
 
-    let character_escape_to_string (esc: character coq_CharacterEscape) : string =
+    let character_escape_to_string (esc: (character, string) coq_CharacterEscape) : ocaml_string =
       match esc with
       | ControlEsc esc -> (match esc with
         | Coq_esc_f -> "\\f"
@@ -53,7 +54,7 @@ module Printer(P: EngineParameters) = struct
         | CodePoint i -> failwith "TODO: pretty-printer -- \\u{codepoint}")
       | IdentityEsc c -> escape c
 
-    let character_class_escape_to_string (esc: character coq_CharacterClassEscape) : string =
+    let character_class_escape_to_string (esc: (character, string) coq_CharacterClassEscape) : ocaml_string =
       match esc with
       | Coq_esc_d -> "\\d"
       | Coq_esc_D -> "\\D"
@@ -64,7 +65,7 @@ module Printer(P: EngineParameters) = struct
       | UnicodeProp _ -> "\\p{...}"
       | UnicodePropNeg _ -> "\\P{...}"
 
-    let quantifier_prefix_to_string (qp: coq_QuantifierPrefix) : string =
+    let quantifier_prefix_to_string (qp: coq_QuantifierPrefix) : ocaml_string =
       match qp with
       | Star -> "*"
       | Plus -> "+"
@@ -73,12 +74,12 @@ module Printer(P: EngineParameters) = struct
       | RepPartialRange (i) -> "{" ^ string_of_int i ^ ",}"
       | RepRange (imin,imax) -> "{" ^ string_of_int imin ^ "," ^ string_of_int imax ^ "}"
 
-    let quantifier_to_string (q: coq_Quantifier) : string =
+    let quantifier_to_string (q: coq_Quantifier) : ocaml_string =
       match q with
       | Greedy (qp) -> quantifier_prefix_to_string qp
       | Lazy (qp) -> quantifier_prefix_to_string qp ^ "?"
 
-    let class_atom_to_string (ca: character coq_ClassAtom) : string =
+    let class_atom_to_string (ca: (character, string) coq_ClassAtom) : ocaml_string =
       match ca with
       | SourceCharacter c -> char_lit_to_string c
       | ClassEsc Coq_esc_b -> "\\b"
@@ -86,7 +87,7 @@ module Printer(P: EngineParameters) = struct
       | ClassEsc (CCharacterClassEsc esc) -> character_class_escape_to_string esc
       | ClassEsc (CCharacterEsc esc) -> character_escape_to_string esc
 
-    let rec range_to_string (r: character coq_ClassRanges) : string =
+    let rec range_to_string (r: (character, string) coq_ClassRanges) : ocaml_string =
     match r with
     | EmptyCR -> ""
     | ClassAtomCR (ca, r) -> (class_atom_to_string ca) ^ (range_to_string r)
@@ -95,26 +96,26 @@ module Printer(P: EngineParameters) = struct
 
     (* Exec result printers *)
 
-    let quoted (str: Unsigned.uint16 list) : string = "'" ^ Encoding.Utf16.list_to_string str ^ "'"
+    let quoted (str: string) : ocaml_string = "'" ^ P.String.to_host str ^ "'"
 
-    let string_range (string_input: string) (single_capture: CaptureRange.coq_type) : string =
-      let { CaptureRange.startIndex = s; CaptureRange.endIndex = e } = single_capture in
+    let string_range (string_input: ocaml_string) (single_capture: Extracted.Notation.CaptureRange.coq_type) : ocaml_string =
+      let { Extracted.Notation.CaptureRange.startIndex = s; Extracted.Notation.CaptureRange.endIndex = e } = single_capture in
       String.sub string_input s (e-s)
 
-    let option_to_string (type a) ?(none="Undefined") ?(some_prefix="") (p: a -> string) (o: a option) : string =
+    let option_to_string (type a) ?(none="Undefined") ?(some_prefix="") (p: a -> ocaml_string) (o: a option) : ocaml_string =
       match o with
       | None -> none
       | Some l -> some_prefix ^ p l
 
-    let pair_to_string (type a b) ?(start="(") ?(sep=",") ?(endd=")") (pa: a -> string) (pb: b -> string) (t: (a * b)) : string =
+    let pair_to_string (type a b) ?(start="(") ?(sep=",") ?(endd=")") (pa: a -> ocaml_string) (pb: b -> ocaml_string) (t: (a * b)) : ocaml_string =
       let (i1, i2) = t in
       start ^ pa i1 ^ sep ^ pb i2 ^ endd
 
-    let keyed_list_to_string (type a b) ?(nil="[]") ?(prefix="\t#") ?(key_sep=":") ?(sep=" ") (pa: a -> string) (pb: b -> string) (l: (a * b) list) : string =
+    let keyed_list_to_string (type a b) ?(nil="[]") ?(prefix="\t#") ?(key_sep=":") ?(sep=" ") (pa: a -> ocaml_string) (pb: b -> ocaml_string) (l: (a * b) list) : ocaml_string =
       if List.length l = 0 then nil else
       prefix ^ String.concat sep (List.map (fun (k, v) -> pa k ^ key_sep ^ pb v) l)
 
-    let indexed_list_to_string (type a) ?(nil="[]") ?(prefix="") ?(key_sep=":") ?(sep=" ") (p: a -> string) (l: a list) : string =
+    let indexed_list_to_string (type a) ?(nil="[]") ?(prefix="") ?(key_sep=":") ?(sep=" ") (p: a -> ocaml_string) (l: a list) : ocaml_string =
       let rec indexed (l: a list) (index: int) : (int * a) list =
         match l with
         | [] -> []
@@ -122,7 +123,7 @@ module Printer(P: EngineParameters) = struct
       in
       keyed_list_to_string ~nil:nil ~prefix:prefix ~key_sep:key_sep ~sep:sep string_of_int p (indexed l 0)
 
-    let exec_array_exotic_to_string (pretty: bool) (a: Extracted.ExecArrayExotic.coq_type) : string =
+    let exec_array_exotic_to_string (pretty: bool) (a: execArrayExotic) : ocaml_string =
       if pretty then
         let zip_with_opt (type a b) (l: a list) (r: b option list option) = match r with
           | None -> List.map (fun l -> (l, None)) l
@@ -143,7 +144,7 @@ module Printer(P: EngineParameters) = struct
             (zip_with_opt a.array a.indices_array)) ::
           (option_to_string ~none:"" ~some_prefix:"Named captures:"
               (keyed_list_to_string ~prefix:"\027[20G# " ~key_sep:"\027[32G: " ~sep:"\n\027[20G# "
-                Encoding.Utf16.list_to_string
+                P.String.to_host
                 (pair_to_string ~start:"" ~sep:"\027[64G" ~endd:""
                   (option_to_string quoted)
                   (option_to_string ~none:"" (pair_to_string string_of_int string_of_int))))
@@ -160,7 +161,7 @@ module Printer(P: EngineParameters) = struct
           ("Named captures:" ^ (
             option_to_string ~none:"\n\tNone" 
               (keyed_list_to_string ~nil:"\n\tNone" ~prefix:"\n\t# " ~key_sep:" : " ~sep:"\n\t# "
-                Encoding.Utf16.list_to_string
+                P.String.to_host
                 (option_to_string quoted))
             a.groups)) ::
           ("Indices:" ^ (
@@ -171,16 +172,9 @@ module Printer(P: EngineParameters) = struct
           ("Named indices:" ^ (
             option_to_string ~none:"\n\tNone" 
               (keyed_list_to_string ~nil:"\n\tNone" ~prefix:"\n\t# " ~key_sep:" : " ~sep:"\n\t# "
-                Encoding.Utf16.list_to_string
+              P.String.to_host
                 (option_to_string ~none:"Undefined" (pair_to_string string_of_int string_of_int)))
             a.indices_groups)) ::
-          (* (option_to_string ~none:"" ~some_prefix:"Named captures:"
-              (keyed_list_to_string ~prefix:"\027[20G# " ~key_sep:"\027[32G: " ~sep:"\n\027[20G# "
-                Encoding.Utf16.list_to_string
-                (pair_to_string ~start:"" ~sep:"\027[64G" ~endd:""
-                  (option_to_string quoted)
-                  (option_to_string ~none:"" (pair_to_string string_of_int string_of_int))))
-            named_captures) :: *)
           []
         ))
   end
@@ -190,10 +184,10 @@ module Printer(P: EngineParameters) = struct
     In strict mode, the regex will be printed as is.
     In non-strict mode, an equivalent regex (through associativity) might be printed.
     Additionally, in non-strict mode, parentheses which are not required by most engines (but are mandated by the spec) are not printed. *)
-  let regex_to_string ?(delimited=true) ?(strict=false) (r: character coq_Regex) : string =
+  let regex_to_string ?(delimited=true) ?(strict=false) (r: (character, string) coq_Regex) : ocaml_string =
     let next (i: int) : int = if strict then i + 1 else i in
-    let prio_if_strict (str: string) (at: int) (current: int) : string = if strict then prio str at current else str in
-    let rec iter (r: character coq_Regex) (current: int) : string =
+    let prio_if_strict (str: ocaml_string) (at: int) (current: int) : ocaml_string = if strict then prio str at current else str in
+    let rec iter (r: (character, string) coq_Regex) (current: int) : ocaml_string =
       match r with
       | Empty -> prio_if_strict "" 3 current
       | Char c -> char_lit_to_string c
@@ -204,12 +198,12 @@ module Printer(P: EngineParameters) = struct
       | AtomEsc (DecimalEsc gid) -> "\\" ^ string_of_int gid
       | AtomEsc (ACharacterClassEsc esc) -> character_class_escape_to_string esc
       | AtomEsc (ACharacterEsc esc) -> character_escape_to_string esc
-      | AtomEsc (GroupEsc name) -> "\\" ^ "k<" ^ Encoding.Utf16.list_to_string name ^ ">"
+      | AtomEsc (GroupEsc name) -> "\\" ^ "k<" ^ P.String.to_host name ^ ">"
       | Disjunction (r1, r2) -> prio ((iter r1 (next 0)) ^ "|" ^ (iter r2 0)) 0 current
       | Quantified (r1, q) -> prio ((iter r1 4) ^ quantifier_to_string q) 3 current
       | Seq (r1, r2) -> prio ((iter r1 (next 1)) ^ (iter r2 1)) 1 current
       | Group (None, r1) -> "(" ^ iter r1 0 ^ ")"
-      | Group (Some name, r1) -> "(?<" ^ Encoding.Utf16.list_to_string name ^  ">" ^ iter r1 0 ^ ")"
+      | Group (Some name, r1) -> "(?<" ^ P.String.to_host name ^  ">" ^ iter r1 0 ^ ")"
       | InputStart -> prio "^" 3 current
       | InputEnd -> prio_if_strict "$" 3 current
       | WordBoundary -> prio_if_strict "\\b" 3 current
@@ -222,19 +216,18 @@ module Printer(P: EngineParameters) = struct
     let res = iter r 0 in
     if delimited then "/" ^ res ^ "/" else res
 
-  let exec_result_to_string ?(pretty=true) (r: character Extracted.execResult) : string =
+  let exec_result_to_string ?(pretty=true) (r: (character, string) Extracted.execResult) : ocaml_string =
     match r with
     | Null _ -> "No match"
     | Exotic (a, _) -> Internal.exec_array_exotic_to_string pretty a
 
-  let flags_to_string (flags: Extracted.RegExpFlags.coq_type) : string =
+  let flags_to_string (flags: Extracted.RegExpFlags.coq_type) : ocaml_string =
     let s = ref "" in
     if (flags.d) then s := "d" ^ !s;
     if (flags.g) then s := "g" ^ !s;
     if (flags.i) then s := "i" ^ !s;
     if (flags.m) then s := "m" ^ !s;
     if (flags.s) then s := "s" ^ !s;
-    if (flags.u) then s := "u" ^ !s;
     if (flags.y) then s := "y" ^ !s;
     !s
 end
