extraction/Extraction.v
@@ -1,4 +1,4 @@
-From Warblre Require Import Base Patterns Semantics Frontend Engine.
+From Warblre Require Import Base Patterns Semantics Frontend Engine Fragments.
 From Coq Require Import ZArith.
 
 From Coq Require Extraction.
@@ -15,19 +15,6 @@ Extract Constant Pos.to_nat => "(fun c -> c)".
 
 Extract Constant host_string => "string".
 
-Extract Constant CodePoint.type => "Encoding.codepoint".
-Extract Constant CodePoint.from_numeric_value => "(fun c -> c)".
-Extract Constant CodeUnit.type => "Unsigned.UInt16.t".
-Extract Constant CodeUnit.is_leading_surrogate => "(fun i -> Encoding.Utf8Utils.is_high_surrogate (Unsigned.UInt16.to_int i))".
-Extract Constant CodeUnit.is_trailing_surrogate => "(fun i -> Encoding.Utf8Utils.is_low_surrogate (Unsigned.UInt16.to_int i))".
-Extract Constant CodeUnit.numeric_value => "Unsigned.UInt16.to_int".
-
-Extract Constant String.type => "Unsigned.UInt16.t list".
-Extract Constant String.eqdec => "(Utils.List.equal Unsigned.UInt16.equal)".
-Extract Constant String.length => "Utils.List.length".
-Extract Constant String.substring => "(fun str s e -> Utils.List.take (e - s) (Utils.List.drop s str))".
-Extract Constant String.codeUnitAt => "(fun str at -> Utils.List.nth str at)".
-
 Extract Constant HexDigit.type => "char".
 Extract Constant HexDigit.to_integer => "Interop.Common.parse_hex".
 
@@ -36,5 +23,5 @@ Extract Constant AsciiLetter.numeric_value => "Char.code".
 
 Extraction Inline Frontend.RegExpInstance.setLastIndex.
 
-Extraction "Extracted.ml"  Engine.Engine.
+Extraction "Extracted.ml" Engine.Engine UnicodeOps.
 
