mechanization/props/EarlyErrors.v
@@ -2,7 +2,7 @@ From Coq Require Import PeanoNat List Lia NArith Program.Equality.
 From Warblre Require Import Tactics List Result Focus Base Characters Patterns Node StaticSemantics.
 
 Section EarlyErrors.
-  Context `{ep: CharacterInstance Σ}.
+  Context `{ep: CharacterInstance Γ Σ}.
     Import Patterns.
 
   Notation hex4digitsValue v := (let (_0, _1, _2, _3) := v in HexDigit.to_integer (_0 :: _1 :: _2 :: _3 :: nil)) (only parsing).
@@ -112,13 +112,13 @@ Section EarlyErrors.
     - let direct_recursion := solve [ exists (fun i => S (f' i)); setoid_rewrite -> Nat.succ_inj_wd; split; try assumption ] in
         destruct rh; try direct_recursion;
         destruct name as [ name | ]; try direct_recursion;
-        cbn; destruct (String.eqdec name (capturingGroupName gn)) eqn:Eq_gs_gn; try direct_recursion.
+        cbn; destruct (name =?= capturingGroupName gn) eqn:Eq_gs_gn; try direct_recursion.
       exists (fun i => if Nat.eqb i 0 then 0 else S (f' (i - 1))).
       split.
       + intros i j H. destruct (Nat.eqb i 0) eqn:Eq_i; destruct (Nat.eqb j 0) eqn:Eq_j; spec_reflector Nat.eqb_spec; subst.
         * reflexivity. * discriminate. * discriminate. * apply Nat.succ_inj in H. specialize H0 with (1 := H). lia.
       + intros [| i] r' ctx'; cbn.
-        * cbn. subst. subst. intros [=<-<-]. exists ctxh. split; reflexivity.
+        * cbn. subst. intros [=<-<-]. exists ctxh. split; reflexivity.
         * rewrite -> List.Indexing.Nat.cons. rewrite -> Nat.sub_0_r. apply H1.
   Qed.
 
@@ -154,7 +154,7 @@ Section EarlyErrors.
     - discriminate.
     - cbn in H. destruct h as [ h_r h_ctx ].
       destruct h_r; try destruct name as [ name | ]; try solve [ cbn in H; apply (IHt' H) ].
-      destruct (String.eqdec name (capturingGroupName gn)).
+      destruct (name =?= capturingGroupName gn).
       + cbn in H. subst. injection H as <-. split.
         * subst. cbn. lia.
         * exists h_ctx. symmetry. assumption.
